TM/Code/SumTM.v
@@ -1,0 +1,148 @@
+Require Import ProgrammingTools MatchSum.
+
+
+
+(**
+If there are two function [f1 : X -> Z] and [f2 : Y -> Z], then there is only one canonical way to define a function [map_sum : X + Y -> Z]. This machine operator takes machines [M1] and [M2] that compute the functions [f] and [g]; and defines a machine [Map_sum] that computes [map_sum]. Alphabets have to be handled with care, to define this machine as general as possible.
+One way would be to let [M1] be a machine over [sigX + sigZ] and [M2] over the alphabet [sigY+sigZ]; and to define [Map_sum] over [sigSum sigX sigY + sigZ], but this is not general enough, as a "client" with an alphabet [sig] would had to give a retract from [sigSum sigX sigY + sigZ] to [sig], but this is in general not possible or to complicated. (Counterexample: there is no retract from [unit+unit] to [unit])
+*)
+
+Section MapSum.
+
+  Variable n : nat.
+  Variable (sigX sigY sigZ : finType) (defX : sigX) (defY : sigY) (defZ : sigZ).
+  Variable (X Y Z : Type) (codX : codable sigX X) (codY : codable sigY Y) (codZ : codable sigZ Z).
+
+  (** The alphabet of the first machine contains [sigX] for the input and [sigZ] for the output, so assume retracts from said alphabets to the alphabet of [sigM1]. *)
+  Variable (sigM1 : finType) (retr_sigX_sigM1 : Retract sigX sigM1) (retr_sigZ_sigM1 : Retract sigZ sigM1).
+  Variable (sigM2 : finType) (retr_sigY_sigM2 : Retract sigY sigM2) (retr_sigZ_sigM2 : Retract sigZ sigM2).
+
+
+  (** We assume an alphabet [sig] of the "mapped" machine. It should at least contain the alphabets of [M1] and [M2]. *)
+  Variable (sig : finType) (retr_sigM1_sig : Retract sigM1 sig) (retr_sigM2_sig : Retract sigM2 sig).
+
+  (** Note that there are now two possible ways how to encode [Z] on [sig]: over the retract from [sigZ] to [sigM1] to [sig], and from [sigZ] to [sigM2] to [sig]. To solve this problem, we assume another retract from [sigZ] to [sig] and copy the result of [M1] or [M2] to this encoding. *)
+  Variable (retr_sigZ_sig : Retract sigZ sig).
+
+  (** The other two retracts from [sigZ] to [sig]: *)
+  Definition retr_sigZ_sig_M1 : Retract sigZ sig := ComposeRetract retr_sigZ_sigM1 retr_sigM1_sig.
+  Definition retr_sigZ_sig_M2 : Retract sigZ sig := ComposeRetract retr_sigZ_sigM2 retr_sigM2_sig.
+
+  (** The input of the "mapped" machine is on [sigSum sigX sigY], which we have to add to the alphabet [sig]. *)
+  Variable (retr_sigSum_sig : Retract (sigSum sigX sigY) sig).
+
+  (** Note that we now have the same problem like above for [sigX] and [sigY]: There are multiple ways how to encode [X] and [Y] on [sig]. We simply have to translate from the alphabet [sigX], which is in [sigSum sigX sigY], to the corresponding alphabet [sigX] by [M1], before calling [M1]. *)
+
+  Definition retr_sigX_sig : Retract sigX sig := ComposeRetract (Retract_sigSum_X _ _) retr_sigSum_sig.
+  Definition retr_sigX_sig_M1 : Retract sigX sig := ComposeRetract retr_sigX_sigM1 retr_sigM1_sig.
+
+  Definition retr_sigY_sig : Retract sigY sig := ComposeRetract (Retract_sigSum_Y _ _) retr_sigSum_sig.
+  Definition retr_sigY_sig_M2 : Retract sigY sig := ComposeRetract retr_sigY_sigM2 retr_sigM2_sig.
+  
+
+  (** The Machines [M1] and [M2] that compute the functions [f1] and [f2]. *)
+  Variable M1 : { M : mTM sigM1^+ (S (S n)) & states M -> unit }.
+  Variable M2 : { M : mTM sigM2^+ (S (S n)) & states M -> unit }.
+
+  Variable f : X -> Z.
+  Variable g : Y -> Z.
+
+  Hypothesis M1_Computes : M1 ⊨ Computes_Rel f.
+  Hypothesis M2_Computes : M2 ⊨ Computes_Rel g.
+
+  (** The mapped function *)
+  Definition map_sum : X + Y -> Z :=
+    fun s => match s with
+          | inl x => f x
+          | inr y => g y
+          end.
+
+  
+  (** I use [Id] here to prevent [TM_Correct] unfolding [ChangeAlphabet], because we want to apply [ChangeAlphabet_Computes] instead. *)
+  Definition MapSum : { M : mTM sig^+ (S (S n)) & states M -> unit } :=
+    If (MatchSum sigX sigY ⇑ _ @ [|Fin0|])
+       (Translate retr_sigX_sig retr_sigX_sig_M1 @ [|Fin0|];; (* Translate [x] to the alphabet of [M1] *)
+        Id (M1 ⇑ _);; (* Call [M1] *)
+        Translate retr_sigX_sig_M1 retr_sigX_sig @ [|Fin0|];; (* Translate [x] back to the "choosen" [sigX] on [sig] *)
+        Translate retr_sigZ_sig_M1 retr_sigZ_sig @ [|Fin1|];; (* Translate the result [z] to the "choosen" [sigZ] on [sig] *)
+        Constr_inl sigX sigY ⇑ _ @ [|Fin0|]) (* Apply the [inl] constructor again to [x], which has been removed by [MatchSum] *)
+       (Translate retr_sigY_sig retr_sigY_sig_M2 @ [|Fin0|];; (* Translate [y] to the alphabet of [M2] *)
+        Id (M2 ⇑ _);; (* Call [M2] *)
+        Translate retr_sigY_sig_M2 retr_sigY_sig @ [|Fin0|];; (* Translate [y] back to the "choosen" [sigY] on [sig] *)
+        Translate retr_sigZ_sig_M2 retr_sigZ_sig @ [|Fin1|];; (* Translate the result [z] to the "choosen" [sigZ] on [sig] *)
+        Constr_inr sigX sigY ⇑ _ @ [|Fin0|]) (* Apply the [inr] constructor again to [y], which has been removed by [MatchSum] *)
+  .
+
+
+  (* TODO: [Translate_Realise] maybe could be registered to [TM_Correct]. *)
+  Lemma MapSum_Computes : MapSum ⊨ Computes_Rel map_sum.
+  Proof.
+    eapply Realise_monotone.
+    { unfold MapSum. repeat TM_Correct.
+      - apply Translate_Realise with (X := X).
+      - apply (ChangeAlphabet_Computes (M1_Computes)).
+      - apply Translate_Realise with (X := X).
+      - apply Translate_Realise with (X := Z).
+      - apply Translate_Realise with (X := Y).
+      - apply (ChangeAlphabet_Computes (M2_Computes)).
+      - apply Translate_Realise with (X := Y).
+      - apply Translate_Realise with (X := Z).
+    }
+    {
+      intros tin ((), tout) H. cbn. intros s HEncS HOut HInt.
+      destruct H; TMSimp. (* Both cases of the [If] are symmetric. *)
+      { (* Then case, i.e. [s = inl x] *)
+        (* give better names... *)
+        rename H into HMatchSum, H1 into HInj1, H0 into HTranslate, H3 into HInj2, H2 into HCompM, H4 into HTranslate'.
+        rename H6 into HInj3, H5 into HTranslate'', H9 into HInj4, H7 into HConstr, H8 into HInj5.
+        (* instantiate the hypothesises.. *)
+        modpon HMatchSum. destruct s as [x|y]; auto. simpl_surject. (* We now know that [s = inl x]. *)
+        modpon HTranslate.
+        modpon HCompM. (* If [modpon] can't solve a premise of a hypothesis, it opens a goal to let the user prove it. *)
+        (* This normally happens automatically, however, [TMSimp] can't handle quantified hypothesises. *)
+        { rewrite HInj2, HInj1; auto; vector_not_in. }
+        { intros i. now rewrite HInj2, HInj1 by vector_not_in. }
+        (* If you want to show the encoding instance somewhere, just [unfold tape_contains] to see it. *)
+        unfold tape_contains in HCompM0, HConstr, HCompM0.
+        (* Instead of the automatic tactic [modpon], you can also specialize the hypothesis manually and call [spec_assert] *)
+        specialize (HTranslate' x); spec_assert HTranslate' by now contains_ext.
+        modpon HTranslate''.
+        { rewrite HInj3 by vector_not_in. contains_ext. }
+        specialize (HConstr x). modpon HConstr.
+        { eapply contains_translate_tau1. rewrite HInj4 by vector_not_in. contains_ext. }
+        (* Now we have solved all hypothesises, time to call [repeat split; eauto]. *)
+        repeat split; cbn; eauto.
+        - now rewrite HInj5 by vector_not_in.
+        - intros i. now rewrite HInj5, HInj4, HInj3 by vector_not_in.
+      }
+      { (* Then case, i.e. [s = iny y], completely symmetric *)
+        (* give better names... *)
+        rename H into HMatchSum, H1 into HInj1, H0 into HTranslate, H3 into HInj2, H2 into HCompM, H4 into HTranslate'.
+        rename H6 into HInj3, H5 into HTranslate'', H9 into HInj4, H7 into HConstr, H8 into HInj5.
+        (* instantiate the hypothesises.. *)
+        modpon HMatchSum. destruct s as [x|y]; auto. simpl_surject. (* We now know that [s = inr y]. *)
+        modpon HTranslate.
+        modpon HCompM. (* If [modpon] can't solve a premise of a hypothesis, it opens a goal to let the user prove it. *)
+        (* This normally happens automatically, however, [TMSimp] can't handle quantified hypothesises. *)
+        { rewrite HInj2, HInj1; auto; vector_not_in. }
+        { intros i. now rewrite HInj2, HInj1 by vector_not_in. }
+        (* If you want to show the encoding instance somewhere, just [unfold tape_contains] to see it. *)
+        unfold tape_contains in HCompM0, HConstr, HCompM0.
+        (* Instead of the automatic tactic [modpon], you can also specialize the hypothesis manually and call [spec_assert] *)
+        specialize (HTranslate' y); spec_assert HTranslate' by now contains_ext.
+        modpon HTranslate''.
+        { rewrite HInj3 by vector_not_in. contains_ext. }
+        specialize (HConstr y). modpon HConstr.
+        { eapply contains_translate_tau1. rewrite HInj4 by vector_not_in. contains_ext. }
+        (* Now we have solved all hypothesises, time to call [repeat split; eauto]. *)
+        repeat split; cbn; eauto.
+        - now rewrite HInj5 by vector_not_in.
+        - intros i. now rewrite HInj5, HInj4, HInj3 by vector_not_in.
+      }
+    }
+    (* Done. *)
+  Qed.
+
+  (* TODO: Runtime. *)
+
+End MapSum.
